

Lecture #3. Exercise

Amplitude Damping Master Equation:

$$\frac{d\rho}{dt} = -i[H, \rho] + \Gamma(\bar{N}+1)\mathcal{D}[\sigma_-]\rho + \Gamma\bar{N}\mathcal{D}[\sigma_+]\rho$$

In our case $H = \frac{\omega}{2}\sigma_z = \frac{\omega}{2} \begin{pmatrix} 1 & 0 \\ 0 & -1 \end{pmatrix}$

$$\rho(t) = \begin{pmatrix} p(t) & \alpha(t) \\ \alpha^*(t) & 1-p(t) \end{pmatrix}$$

Recall $\mathcal{D}[L]\rho = L\rho L^\dagger - \frac{1}{2}\{L^\dagger L, \rho\}$

and $\sigma_+ = \begin{pmatrix} 0 & 1 \\ 0 & 0 \end{pmatrix}$; $\sigma_- = \begin{pmatrix} 0 & 0 \\ 1 & 0 \end{pmatrix}$

Lets perform matrix multiplication separately for each term.

- $-i[H, \rho] = -iH\rho + i\rho H =$

$$= -i\frac{\omega}{2} \begin{pmatrix} 1 & 0 \\ 0 & -1 \end{pmatrix} \begin{pmatrix} p & \alpha \\ \alpha^* & 1-p \end{pmatrix} + i\frac{\omega}{2} \begin{pmatrix} p & \alpha \\ \alpha^* & 1-p \end{pmatrix} \begin{pmatrix} 1 & 0 \\ 0 & -1 \end{pmatrix} =$$

$$= -i\frac{\omega}{2} \begin{pmatrix} p & \alpha \\ -\alpha^* & p-1 \end{pmatrix} + i\frac{\omega}{2} \begin{pmatrix} p & -\alpha \\ \alpha^* & p-1 \end{pmatrix} = -i\frac{\omega}{2} \begin{pmatrix} 0 & 2\alpha \\ -2\alpha^* & 0 \end{pmatrix} =$$

$$= -i\omega \begin{pmatrix} 0 & \alpha \\ \alpha^* & 0 \end{pmatrix}$$

- $\mathcal{D}[\sigma_-]\rho = \sigma_- \rho \sigma_-^\dagger - \frac{1}{2}\{\sigma_-^\dagger \sigma_-, \rho\} = \left\{ \sigma_-^\dagger \sigma_- = \begin{pmatrix} 0 & 1 \\ 0 & 0 \end{pmatrix} \begin{pmatrix} 0 & 0 \\ 1 & 0 \end{pmatrix} = \begin{pmatrix} 1 & 0 \\ 0 & 0 \end{pmatrix} \right\} =$

$$= \begin{pmatrix} 0 & 0 \\ 1 & 0 \end{pmatrix} \begin{pmatrix} p & \alpha \\ \alpha^* & 1-p \end{pmatrix} \begin{pmatrix} 0 & 1 \\ 0 & 0 \end{pmatrix} - \frac{1}{2} \begin{pmatrix} 1 & 0 \\ 0 & 0 \end{pmatrix} \begin{pmatrix} p & \alpha \\ \alpha^* & p \end{pmatrix} - \frac{1}{2} \begin{pmatrix} p & \alpha \\ \alpha^* & p \end{pmatrix} \begin{pmatrix} 1 & 0 \\ 0 & 0 \end{pmatrix} =$$

$$= \begin{pmatrix} 0 & 0 \\ p & \alpha \end{pmatrix} \begin{pmatrix} 0 & 1 \\ 0 & 0 \end{pmatrix} - \frac{1}{2} \begin{pmatrix} p & \alpha \\ 0 & 0 \end{pmatrix} - \frac{1}{2} \begin{pmatrix} p & 0 \\ \alpha^* & 0 \end{pmatrix} =$$

$$= \begin{pmatrix} 0 & 0 \\ 0 & p \end{pmatrix} - \frac{1}{2} \begin{pmatrix} 2p & \alpha \\ \alpha^* & 0 \end{pmatrix} = \begin{pmatrix} -p & -\alpha/2 \\ -\alpha^*/2 & p \end{pmatrix}$$

$$\begin{aligned}
\bullet \mathcal{L}[\bar{\psi}]p &= \bar{\psi}p\bar{\psi}^\dagger - \frac{1}{2}\{\bar{\psi}^\dagger\bar{\psi}, p\} = \left\{ \bar{\psi}^\dagger\bar{\psi} = \begin{pmatrix} 0 & 0 \\ 1 & 0 \end{pmatrix} \begin{pmatrix} 0 & 1 \\ 0 & 0 \end{pmatrix} = \begin{pmatrix} 0 & 0 \\ 0 & 1 \end{pmatrix} \right\} = \\
&= \begin{pmatrix} 0 & 1 \\ 0 & 0 \end{pmatrix} \begin{pmatrix} p & \alpha \\ \alpha^* & 1-p \end{pmatrix} \begin{pmatrix} 0 & 0 \\ 1 & 0 \end{pmatrix} - \frac{1}{2} \begin{pmatrix} 0 & 0 \\ 0 & 1 \end{pmatrix} \begin{pmatrix} p & \alpha \\ \alpha^* & 1-p \end{pmatrix} - \frac{1}{2} \begin{pmatrix} p & \alpha \\ \alpha^* & 1-p \end{pmatrix} \begin{pmatrix} 0 & 0 \\ 0 & 1 \end{pmatrix} = \\
&= \begin{pmatrix} \alpha^* & 1-p \\ 0 & 0 \end{pmatrix} \begin{pmatrix} 0 & 0 \\ 1 & 0 \end{pmatrix} - \frac{1}{2} \begin{pmatrix} 0 & 0 \\ \alpha^* & 1-p \end{pmatrix} - \frac{1}{2} \begin{pmatrix} 0 & \alpha \\ 0 & 1-p \end{pmatrix} = \\
&= \begin{pmatrix} 1-p & 0 \\ 0 & 0 \end{pmatrix} - \begin{pmatrix} 0 & \alpha/2 \\ \alpha^*/2 & 1-p \end{pmatrix} = \begin{pmatrix} 1-p & -\alpha/2 \\ -\alpha^*/2 & p-1 \end{pmatrix}
\end{aligned}$$

Combining everything together,

$$\frac{d\bar{\psi}}{dt} = \begin{pmatrix} 0 & -i\omega\alpha \\ i\omega\alpha^* & 0 \end{pmatrix} + \Gamma(\bar{N}+1) \begin{pmatrix} -p & -\alpha/2 \\ -\alpha^*/2 & p \end{pmatrix} + \Gamma\bar{N} \begin{pmatrix} 1-p & -\alpha/2 \\ -\alpha^*/2 & p-1 \end{pmatrix}$$

$$\frac{d\bar{\psi}}{dt} = \begin{pmatrix} d\bar{p}/dt & d\alpha/dt \\ d\alpha^*/dt & -dp/dt \end{pmatrix}$$

$$\begin{aligned}
\text{So, } \frac{dp}{dt} &= -\Gamma(\bar{N}+1)p + \Gamma\bar{N}(1-p) = -\Gamma\bar{N}p - \Gamma p + \Gamma\bar{N} - \Gamma\bar{N}p = \\
&= \Gamma\bar{N} - \Gamma(2\bar{N}+1)p
\end{aligned}$$

$$\begin{aligned}
\frac{d\alpha}{dt} &= -i\omega\alpha - \Gamma(\bar{N}+1)\frac{\alpha}{2} - \Gamma\bar{N}\frac{\alpha}{2} = \\
&= -i\omega\alpha - \frac{\Gamma}{2}(2\bar{N}+1)\alpha
\end{aligned}$$

$$\boxed{\frac{dp}{dt} = \Gamma\bar{N} - \Gamma(2\bar{N}+1)p} \quad (1)$$

$$\boxed{\frac{d\alpha}{dt} = -i\omega\alpha - \frac{\Gamma}{2}(2\bar{N}+1)\alpha} \quad (2)$$

The solution for (2) is $\alpha(t) = e^{-[i\omega + \frac{\Gamma}{2}(2\bar{N}+1)]t}$

Let $\gamma = \Gamma(2\bar{N}+1)$, then $\alpha(t) = e^{-[i\omega + \gamma/2]t}$

(1) takes the form $\frac{dp}{dt} = \Gamma\bar{N} - \gamma p$

The solution for (1) is $p(t) = e^{-\gamma t} p(0) + \int_0^t dt' e^{-\gamma(t-t')} \Gamma \bar{N}$

After integration $p(t) = e^{-\gamma t} p(0) + \frac{\bar{N}}{2\bar{N}+1} (1 - e^{-\gamma t})$

So,

$$\begin{aligned} p(t) &= e^{-\gamma t} p(0) + \frac{\bar{N}}{2\bar{N}+1} (1 - e^{-\gamma t}) \\ \alpha(t) &= e^{-[i\omega + \gamma/2]t} \end{aligned}$$

- $T_1 = \frac{1}{\gamma} = \frac{1}{\Gamma(2\bar{N}+1)} \quad \text{for } T \neq 0K$